src/basic/FStarC.Options.fsti
@@ -339,6 +339,7 @@ val locate_ocaml                : unit    -> ML bool
 val locate_file                 : unit    -> ML (option string)
 
 val locate_z3                   : unit    -> ML (option string)
+val install_lib                 : unit    -> ML bool
 
 val read_krml_file              : unit    -> ML (option string)
 
